Veritas.MerkleVerifier.fst
@@ -6,6 +6,8 @@
 module Veritas.MerkleVerifier
 
 open FStar.Seq
+open FStar.Classical
+open Veritas.SeqLast
 open Veritas.Memory
 open Veritas.Merkle
 
@@ -84,7 +86,8 @@ let verifier_step (e:verifier_log_entry) (vs:verifier_state): Tot verifier_state
         else 
           Failed
     | Evict a -> 
-        if cache_contains cache a then
+        if is_merkle_root a then Failed
+        else if cache_contains cache a then
           Valid (cache_evict a cache)
         else
           Failed
@@ -109,3 +112,141 @@ let init_cache:verifier_cache =
 let verifier (l:verifier_log): Tot verifier_state = 
   verifier_aux l (Valid init_cache)
 
+type vl_index (l:verifier_log) = seq_index l
+
+let is_evict (l:verifier_log) (i:vl_index l): Tot bool =
+  Evict? (index l i)
+
+let evict_addr (l:verifier_log) (i:vl_index l{is_evict l i}): Tot merkle_addr = 
+  Evict?.a (index l i)
+
+let verifiable (l:verifier_log): Tot bool = 
+  Valid? (verifier l)
+
+type verifiable_log = l:verifier_log{verifiable l}
+
+let rec verifiable_implies_prefix_verifiable (l:verifiable_log) (i:nat{i <= length l}):
+  Lemma (requires (True))
+        (ensures (verifiable (slice l 0 i)))
+        (decreases (length l)) = 
+  let n = length l in
+  if n = 0 then ()
+  else if i = n then ()
+  else verifiable_implies_prefix_verifiable (slice l 0 (n - 1)) i    
+
+let evict_payload (l:verifiable_log) (i:vl_index l{is_evict l i}): 
+  Tot (merkle_payload_of_addr (evict_addr l i)) =
+  verifiable_implies_prefix_verifiable l (i + 1);
+  verifiable_implies_prefix_verifiable l i;
+  let a = evict_addr l i in
+  let l'' = slice l 0 i in
+  let vs'' = verifier l'' in    
+  Some?.v ((Valid?.vc vs'') a)
+
+let is_evict_of_addr (a:merkle_addr) (e:verifier_log_entry) = 
+  Evict? e && Evict?.a e = a
+
+let last_evict (l:verifier_log) (a:merkle_addr):
+  Tot (option (i:vl_index l{is_evict_of_addr a (index l i)})) = 
+  let f = is_evict_of_addr a in
+  let optwi = last_index l f in
+  if None? optwi then None
+  else 
+    let wi = Some?.v optwi in
+    (last_index_correct1 l f; Some wi)
+
+let is_add (l:verifier_log) (i:vl_index l) = 
+  Add? (index l i)
+
+let add_addr (l:verifier_log) (i:vl_index l{is_add l i}): Tot merkle_addr = 
+  Add?.a (index l i)
+
+let add_payload (l:verifier_log) (i:vl_index l {is_add l i}): Tot merkle_payload =
+  Add?.v (index l i)
+
+let prev_evict_of_add (l:verifier_log) (i:vl_index l{is_add l i}):
+  Tot (option (j:vl_index l{j < i && is_evict l j && add_addr l i = evict_addr l j})) = 
+  let l' = slice l 0 i in
+  let a = add_addr l i in 
+  let optj = last_evict l' a in
+  if None? optj then None
+  else
+    let j = Some?.v optj in 
+    (
+      lemma_len_slice l 0 i;
+      lemma_index_slice l 0 i j;
+      Some j
+    )
+
+let has_prev_evict (l:verifier_log) (i:vl_index l{is_add l i}): Tot bool = 
+  Some? (prev_evict_of_add l i)
+
+let has_no_prev_evict (l:verifier_log) (i:vl_index l{is_add l i}): Tot bool =
+  None? (prev_evict_of_add l i)
+
+let rec project_memory_log (l:verifier_log): 
+  Tot memory_op_log (decreases (length l)) = 
+  let n = length l in
+  if n = 0 then empty
+  else 
+    let l' = slice l 0 (n - 1) in
+    let ml' = project_memory_log l' in
+    let e = index l (n - 1) in
+    match e with
+    | MemoryOp o -> append ml' (create 1 o)
+    | _ -> ml'
+
+type evict_add_consistent (l:verifiable_log) = 
+  u:unit{forall (i:vl_index l). 
+    is_add l i /\ is_merkle_leaf (add_addr l i) ==> 
+    has_no_prev_evict l i && add_payload l i = MkLeaf Null \/
+    has_prev_evict l i && 
+    add_payload l i = evict_payload l (Some?.v (prev_evict_of_add l i))
+    }
+
+let cache_at_end (l:verifiable_log): Tot verifier_cache = 
+  Valid?.vc (verifier l)
+
+let last_write_value_or_null (l:verifiable_log) (ma:merkle_leaf_addr): Tot merkle_payload =
+  let ml = project_memory_log l in
+  let a = merkle_leaf_to_addr ma in
+  if has_some_write ml a then
+    MkLeaf (last_write_value ml a)
+  else
+    MkLeaf Null
+      
+let rec eac_implies_cache_is_last_write (l:verifiable_log) (a:merkle_leaf_addr):
+  Lemma (requires (evict_add_consistent l))
+        (ensures (cache_contains (cache_at_end l) a ==> 
+                  Some?.v ((cache_at_end l) a) = last_write_value_or_null l a))
+        (decreases (length l)) = admit()
+
+let rec eac_implies_read_last_write (l:verifiable_log):
+  Lemma (requires (evict_add_consistent l))
+        (ensures (
+
+let rec evict_add_consistency_implies_rw_consistency (l:verifiable_log):
+  Lemma (requires (forall (i:vl_index l). 
+                     is_add l i /\ is_merkle_leaf (add_addr l i)  ==> 
+                       has_no_prev_evict l i && add_payload l i = MkLeaf Null \/
+                       has_prev_evict l i && 
+                       add_payload l i = evict_payload l (Some?.v (prev_evict_of_add l i))))
+        (ensures (rw_consistent (project_memory_log l)))
+        (decreases (length l)) = 
+  let n = length l in
+  if n = 0 then ()
+  else 
+    let l' = slice l 0 (n - 1) in
+    let e = index l (n - 1) in
+    let aux (i:vl_index l'):
+      Lemma (is_add l' i /\ is_merkle_leaf (add_addr l' i) ==>
+             has_no_prev_evict l' i && add_payload l' i = MkLeaf Null \/
+             has_prev_evict l' i && 
+             add_payload l' i = evict_payload l (Some?.v (prev_evict_of_add l' i))) = admit () in
+    forall_intro aux; 
+    verifiable_implies_prefix_verifiable l (n - 1);
+    evict_add_consistency_implies_rw_consistency l';
+    match e with
+    | 
+    admit()
+  
